Instantiator.v
@@ -2,23 +2,42 @@ Require Import ObcToClight.Interface.
 Require Import Ident.
 Require Import Operators.
 Require Import Clocks.
+Require Import Stream.
 
 Module OpAux := OperatorsAux Op.
-Module Clks := ClocksFun Ids. 
+Module Clks := ClocksFun Ids.
+Module Str := StreamFun Op OpAux.
 
-Require Import Coq.ZArith.BinInt.
+Require Import NLustre.NLExprSyntax.
+Require Import NLustre.NLExprSemantics.
+
+Module ExprSyn := NLExprSyntaxFun Op.
+Module ExprSem := NLExprSemanticsFun Ids Op OpAux Clks ExprSyn Str.
 
 Require Import NLustre.
+Require Import SyBloc.
+
+Module NL := NLustreFun Ids Op OpAux Clks ExprSyn Str ExprSem.
+Module SB := SyBlocFun Ids Op OpAux Clks ExprSyn Str ExprSem NL.Syn NL.IsF.
+
+Require Import Coq.ZArith.BinInt.
+Require Import NLustreToSyBloc.Translation.
+Require Import NLustreToSyBloc.Correctness.
+
+Module NL2SB := TranslationFun Ids Op Clks ExprSyn NL.Syn SB.Syn NL.Mem.
+Module NL2SBCorr := CorrectnessFun Ids Op OpAux Clks ExprSyn Str ExprSem NL SB NL2SB.
+
 Require Import Obc.
-Require Import NLustreToObc.Translation.
-Require Import NLustreToObc.Correctness.
-Require Import NLustreToObc.Fusible.
 
-Module NL := NLustreFun Ids Op OpAux Clks.
 Module Obc := ObcFun Ids Op OpAux.
-Module Mem := MemoriesFun Ids Op Clks NL.Syn.
-Module Trans := TranslationFun Ids Op OpAux Clks NL.Syn Obc.Syn Mem.
-Module Typ := NLustreToObc.NLObcTyping.NLObcTypingFun Ids Op OpAux Clks NL Obc Mem Trans.
-Module Corr := NLustreToObc.Correctness.CorrectnessFun Ids Op OpAux Clks NL Obc Mem Trans Typ.
-Module Fusible := NLustreToObc.Fusible.FusibleFun Ids Op OpAux Clks NL Obc Trans.
 
+Require Import SyBlocToObc.Translation.
+Require Import SyBlocToObc.SBMemoryCorres.
+Require Import SyBlocToObc.Correctness.
+(* Require Import NLustreToObc.Fusible. *)
+
+Module SB2Obc := TranslationFun Ids Op OpAux Clks ExprSyn SB.Syn Obc.Syn.
+Module MemCorres := SBMemoryCorresFun Ids Op Clks ExprSyn SB.Syn SB.Last.
+Module SB2ObcCorr := CorrectnessFun Ids Op OpAux Clks ExprSyn Str ExprSem NL.Syn NL.IsF SB Obc SB2Obc MemCorres.
+
+(* Module Fusible := NLustreToObc.Fusible.FusibleFun Ids Op OpAux Clks NL Obc Trans. *)
