NLustre.v
@@ -14,22 +14,24 @@ Require Export NLustre.WellFormed.
 Require Export NLustre.Ordered.
 Require Export NLustre.NoDup.
 Require Export NLustre.NLClocking.
+Require Export NLustre.NLClockingSemantics.
 Require Export NLustre.NLTyping.
 Require Export NLustre.NLSchedule.
 
 Require Import Velus.Common.
 
 Module Type NLUSTRE
-       (Ids   : IDS)
-       (Op    : OPERATORS)
-       (OpAux : OPERATORS_AUX Op)
-       (Clks  : CLOCKS Ids).
-  Declare Module Export ExprSyn: NLEXPRSYNTAX        Op.
+       (Ids    : IDS)
+       (Op     : OPERATORS)
+       (OpAux  : OPERATORS_AUX       Op)
+       (Clks   : CLOCKS         Ids)
+       (ExprSyn: NLEXPRSYNTAX        Op)
+       (Str    : STREAM              Op OpAux)
+       (ExprSem: NLEXPRSEMANTICS Ids Op OpAux Clks ExprSyn Str).
+
   Declare Module Export Syn    : NLSYNTAX        Ids Op       Clks ExprSyn.
-  Declare Module Export Str    : STREAM              Op OpAux.
   Declare Module Export Ord    : ORDERED         Ids Op       Clks ExprSyn Syn.
   Declare Module Export IsF    : ISFREE          Ids Op       Clks ExprSyn Syn.
-  Declare Module Export ExprSem: NLEXPRSEMANTICS Ids Op OpAux Clks ExprSyn     Str.
   Declare Module Export Sem    : NLSEMANTICS     Ids Op OpAux Clks ExprSyn Syn Str Ord ExprSem.
   Declare Module Export Typ    : NLTYPING        Ids Op       Clks ExprSyn Syn.
   Declare Module Export Mem    : MEMORIES        Ids Op       Clks ExprSyn Syn.
@@ -37,12 +39,12 @@ Module Type NLUSTRE
   Declare Module Export IsV    : ISVARIABLE      Ids Op       Clks ExprSyn Syn                     Mem IsD.
   Declare Module Export NoD    : NODUP           Ids Op       Clks ExprSyn Syn                     Mem IsD IsV.
   Declare Module Export WeF    : WELLFORMED      Ids Op       Clks ExprSyn Syn     Ord             Mem IsD IsV IsF NoD.
-  Declare Module Export MemSem : MEMSEMANTICS    Ids Op OpAux Clks ExprSyn Syn Str Ord ExprSem Sem Mem IsD IsV IsF NoD WeF.
-  Declare Module Export Clo    : NLCLOCKING      Ids Op       Clks ExprSyn Syn                     Mem IsD     IsF.
-  Declare Module Export CloSem : NLCLOCKINGSEMANTICS Ids Op OpAux Clks ExprSyn SynNL
-                                                     Str Ord ExprSem SemNL Mem IsD  IsF NLClk.
+  Declare Module Export MemSem : MEMSEMANTICS    Ids Op OpAux Clks ExprSyn Syn Str Ord ExprSem Sem Mem IsD IsV IsF NoD.
+  Declare Module Export Clo    : NLCLOCKING      Ids Op       Clks ExprSyn Syn     Ord             Mem IsD     IsF.
+  Declare Module Export CloSem : NLCLOCKINGSEMANTICS Ids Op OpAux Clks ExprSyn Syn
+                                                     Str Ord ExprSem Sem Mem IsD  IsF Clo.
 
-  Declare Module Scheduler     : NLSCHEDULE      Ids Op OpAux Clks ExprSyn Syn Str Ord ExprSem Sem Mem IsD     IsF          Typ Clo.
+  Declare Module Scheduler     : NLSCHEDULE      Ids Op OpAux Clks ExprSyn Syn Ord IsF Str Mem IsD ExprSem Sem Typ Clo.
 
 End NLUSTRE.
 
@@ -51,13 +53,13 @@ Module NLustreFun
        (Op    : OPERATORS)
        (OpAux : OPERATORS_AUX Op)
        (Clks  : CLOCKS Ids)
-       <: NLUSTRE Ids Op OpAux Clks.
-  Module Export ExprSyn := NLExprSyntaxFun        Op.
+       (ExprSyn: NLEXPRSYNTAX  Op)
+       (Str    : STREAM              Op OpAux)
+       (ExprSem: NLEXPRSEMANTICS Ids Op OpAux Clks ExprSyn Str)
+       <: NLUSTRE Ids Op OpAux Clks ExprSyn Str ExprSem.
   Module Export Syn     := NLSyntaxFun        Ids Op       Clks ExprSyn.
-  Module Export Str     := StreamFun              Op OpAux.
   Module Export Ord     := OrderedFun         Ids Op       Clks ExprSyn Syn.
   Module Export IsF     := IsFreeFun          Ids Op       Clks ExprSyn Syn.
-  Module Export ExprSem := NLExprSemanticsFun Ids Op OpAux Clks ExprSyn     Str.
   Module Export Sem     := NLSemanticsFun     Ids Op OpAux Clks ExprSyn Syn Str Ord ExprSem.
   Module Export Typ     := NLTypingFun        Ids Op       Clks ExprSyn Syn.
   Module Export Mem     := MemoriesFun        Ids Op       Clks ExprSyn Syn.
@@ -65,11 +67,11 @@ Module NLustreFun
   Module Export IsV     := IsVariableFun      Ids Op       Clks ExprSyn Syn                     Mem IsD.
   Module Export NoD     := NoDupFun           Ids Op       Clks ExprSyn Syn                     Mem IsD IsV.
   Module Export WeF     := WellFormedFun      Ids Op       Clks ExprSyn Syn     Ord             Mem IsD IsV IsF NoD.
-  Module Export MemSem  := MemSemanticsFun    Ids Op OpAux Clks ExprSyn Syn Str Ord ExprSem Sem Mem IsD IsV IsF NoD WeF.
-  Module Export Clo     := NLClockingFun      Ids Op       Clks ExprSyn Syn                     Mem IsD     IsF.
-  Module Export CloSem  := NLClockingSemanticsFun Ids Op OpAux Clks ExprSyn SynNL
-                                                  Str Ord ExprSem SemNL Mem IsD  IsF Clo.
+  Module Export MemSem  := MemSemanticsFun    Ids Op OpAux Clks ExprSyn Syn Str Ord ExprSem Sem Mem IsD IsV IsF NoD.
+  Module Export Clo     := NLClockingFun      Ids Op       Clks ExprSyn Syn     Ord             Mem IsD     IsF.
+  Module Export CloSem  := NLClockingSemanticsFun Ids Op OpAux Clks ExprSyn Syn
+                                                  Str Ord ExprSem Sem Mem IsD  IsF Clo.
 
-  Module Scheduler      := NLScheduleFun      Ids Op OpAux Clks ExprSyn Syn Str Ord ExprSem Sem Mem IsD IsF              Typ Clo.
+  Module Scheduler      := NLScheduleFun      Ids Op OpAux Clks ExprSyn Syn Ord IsF Str Mem IsD ExprSem Sem Typ Clo.
 
 End NLustreFun.
