SyBloc.v
@@ -1,0 +1,64 @@
+Require Import Velus.Common.
+Require Import Velus.Operators.
+Require Import Velus.Clocks.
+Require Export Velus.NLustre.Stream.
+Require Import Velus.NLustre.NLExprSyntax.
+Require Import Velus.SyBloc.SBSyntax.
+Require Import Velus.SyBloc.SBIsBlock.
+Require Import Velus.SyBloc.SBOrdered.
+Require Import Velus.NLustre.NLExprSemantics.
+Require Import Velus.SyBloc.SBSemantics.
+Require Import Velus.SyBloc.SBIsLast.
+Require Import Velus.SyBloc.SBIsVariable.
+Require Import Velus.SyBloc.SBIsDefined.
+Require Import Velus.NLustre.NLSyntax.
+Require Import Velus.NLustre.IsFree.
+Require Import Velus.SyBloc.SBIsFree.
+Require Import Velus.SyBloc.SBWellDefined.
+
+Module Type SYBLOC
+       (Ids    : IDS)
+       (Op     : OPERATORS)
+       (OpAux  : OPERATORS_AUX       Op)
+       (Clks   : CLOCKS          Ids)
+       (ExprSyn: NLEXPRSYNTAX        Op)
+       (Str    : STREAM              Op OpAux)
+       (ExprSem: NLEXPRSEMANTICS Ids Op OpAux Clks ExprSyn Str)
+       (SynNL  : NLSYNTAX        Ids Op       Clks ExprSyn)
+       (FreeNL : ISFREE          Ids Op       Clks ExprSyn     SynNL).
+
+  Declare Module Export Syn  : SBSYNTAX      Ids Op       Clks ExprSyn.
+  Declare Module Export Block: SBISBLOCK     Ids Op       Clks ExprSyn Syn.
+  Declare Module Export Ord  : SBORDERED     Ids Op       Clks ExprSyn Syn Block.
+  Declare Module Export Sem  : SBSEMANTICS   Ids Op OpAux Clks ExprSyn Syn Block Ord Str ExprSem.
+  Declare Module Export Last : SBISLAST      Ids Op       Clks ExprSyn Syn.
+  Declare Module Export Var  : SBISVARIABLE  Ids Op       Clks ExprSyn Syn.
+  Declare Module Export Def  : SBISDEFINED   Ids Op       Clks ExprSyn Syn Var Last.
+  Declare Module Export Free : SBISFREE      Ids Op       Clks ExprSyn Syn SynNL FreeNL.
+  Declare Module Export Wdef : SBWELLDEFINED Ids Op       Clks ExprSyn Syn Block Ord Var Last Def SynNL FreeNL Free.
+
+End SYBLOC.
+
+Module SyBlocFun
+       (Ids    : IDS)
+       (Op     : OPERATORS)
+       (OpAux  : OPERATORS_AUX Op)
+       (Clks   : CLOCKS    Ids)
+       (ExprSyn: NLEXPRSYNTAX  Op)
+       (Str    : STREAM              Op OpAux)
+       (ExprSem: NLEXPRSEMANTICS Ids Op OpAux Clks ExprSyn Str)
+       (SynNL  : NLSYNTAX  Ids Op Clks ExprSyn)
+       (FreeNL : ISFREE    Ids Op Clks ExprSyn SynNL)
+<: SYBLOC Ids Op OpAux Clks ExprSyn Str ExprSem SynNL FreeNL.
+
+  Module Export Syn   := SBSyntaxFun      Ids Op       Clks ExprSyn.
+  Module Export Block := SBIsBlockFun     Ids Op       Clks ExprSyn Syn.
+  Module Export Ord   := SBOrderedFun     Ids Op       Clks ExprSyn Syn Block.
+  Module Export Sem   := SBSemanticsFun   Ids Op OpAux Clks ExprSyn Syn Block Ord Str ExprSem.
+  Module Export Last  := SBIsLastFun      Ids Op       Clks ExprSyn Syn.
+  Module Export Var   := SBIsVariableFun  Ids Op       Clks ExprSyn Syn.
+  Module Export Def   := SBIsDefinedFun   Ids Op       Clks ExprSyn Syn Var Last.
+  Module Export Free  := SBIsFreeFun      Ids Op       Clks ExprSyn Syn SynNL FreeNL.
+  Module Export Wdef  := SBWellDefinedFun Ids Op       Clks ExprSyn Syn Block Ord Var Last Def SynNL FreeNL Free.
+
+End SyBlocFun.
